Misc clean up in counter.

F_mu_ref_par/examples/counter.v
@@ -4,14 +4,43 @@ From iris_logrel.F_mu_ref_par Require Import lang examples.lock typing
      soundness_binary context_refinement.
 Import uPred.
 
+Definition CG_increment (x : expr) : expr :=
+  Lam (Store x.[ren (+ 2)] (BinOp Add (♯ 1) (Load x.[ren (+ 2)]))).
+
+Definition CG_locked_increment (x l : expr) : expr :=
+  with_lock (CG_increment x) l.
+Definition CG_locked_incrementV (x l : expr) : val :=
+  with_lockV (CG_increment x) l.
+
+Definition counter_read (x : expr) : expr := Lam (Load x.[ren (+2)]).
+Definition counter_readV (x : expr) : val := LamV (Load x.[ren (+2)]).
+
+Definition CG_counter_body (x l : expr) : expr :=
+  Pair (CG_locked_increment x l) (counter_read x).
+Definition CG_counter : expr :=
+  App
+    (Lam $ App (Lam (CG_counter_body (Var 1) (Var 3)))
+               (Alloc (♯ 0)))
+    newlock.
+
+Definition FG_increment (x : expr) : expr :=
+  Lam $ App
+    (Lam $
+      (* try increment *)
+      If (CAS x.[ren (+4)] (Var 1) (BinOp Add (♯ 1) (Var 1)))
+          Unit (* increment succeeds we return unit *)
+          (App (Var 2) (Var 3)) (* increment fails, we try again *))
+    (Load x.[ren (+2)]) (* read the counter *).
+Definition FG_counter_body (x : expr) : expr :=
+  Pair (FG_increment x) (counter_read x).
+Definition FG_counter : expr :=
+  App (Lam (FG_counter_body (Var 1))) (Alloc (♯ 0)).
+
 Section CG_Counter.
   Context {Σ : gFunctors} {iS : cfgSG Σ} {iI : heapIG Σ}.
   Implicit Types Δ : varC -n> bivalC -n> iPropG lang Σ.
 
   (* Coarse-grained increment *)
-  Definition CG_increment (x : expr) : expr :=
-    Lam ((Store x.[ren (+ 2)] (BinOp Add (♯ 1) (Load x.[ren (+ 2)])))).
-
   Lemma CG_increment_type x Γ :
     typed Γ x (Tref TNat) →
     typed Γ (CG_increment x) (TArrow TUnit TUnit).
@@ -56,11 +85,6 @@ Section CG_Counter.
 
   Global Opaque CG_increment.
 
-  Definition CG_locked_increment (x l : expr) :=
-    with_lock (CG_increment x) l.
-  Definition CG_locked_incrementV (x l : expr) : val :=
-    with_lockV (CG_increment x) l.
-
   Lemma CG_locked_increment_to_val x l :
     to_val (CG_locked_increment x l) = Some (CG_locked_incrementV x l).
   Proof. by rewrite with_lock_to_val. Qed.
@@ -98,91 +122,76 @@ Section CG_Counter.
   Lemma steps_CG_locked_increment N E ρ j K x n l :
     nclose N ⊆ E →
     Spec_ctx N ρ ★ x ↦ₛ (♯v n) ★ l ↦ₛ (♭v false)
-               ★ j ⤇ fill K (App
-                                (CG_locked_increment (Loc x) (Loc l)) Unit)
-      ={E}=> j ⤇ fill K Unit ★ x ↦ₛ (♯v S n) ★ l ↦ₛ (♭v false).
+      ★ j ⤇ fill K (App (CG_locked_increment (Loc x) (Loc l)) Unit)
+    ={E}=> j ⤇ fill K Unit ★ x ↦ₛ (♯v S n) ★ l ↦ₛ (♭v false).
   Proof.
     iIntros {HNE} "[#Hspec [Hx [Hl Hj]]]".
     iPvs (steps_with_lock
             _ _ _ j K _ _ _ _ UnitV UnitV _ _ with "[Hj Hx Hl]") as "Hj"; last done.
     - iIntros {K'} "[#Hspec [Hx Hj]]".
       iApply steps_CG_increment; first done. iFrame "Hspec Hj Hx"; trivial.
-    - iFrame "Hspec Hj Hx"; trivial.
+    - by iFrame "Hspec Hj Hx".
       Unshelve. all: trivial.
   Qed.
 
   Global Opaque CG_locked_increment.
 
-  Definition counter_read (x : expr) : expr := (Lam (Load x.[ren (+2)])).
-  Definition counter_readV (x : expr) : val := (LamV (Load x.[ren (+2)])).
-
-  Lemma counter_read_to_val x: to_val (counter_read x) = Some (counter_readV x).
+  Lemma counter_read_to_val x : to_val (counter_read x) = Some (counter_readV x).
   Proof. trivial. Qed.
 
-  Lemma counter_read_of_val x: of_val (counter_readV x) = counter_read x.
+  Lemma counter_read_of_val x : of_val (counter_readV x) = counter_read x.
   Proof. trivial. Qed.
 
   Global Opaque counter_readV.
 
   Lemma counter_read_type x Γ :
-    typed Γ x (Tref TNat) →
-    typed Γ (counter_read x) (TArrow TUnit TNat).
+    typed Γ x (Tref TNat) → typed Γ (counter_read x) (TArrow TUnit TNat).
   Proof.
     intros H1. repeat econstructor.
     eapply (context_weakening [_; _]); trivial.
   Qed.
 
   Lemma counter_read_closed (x : expr) :
-    (∀ f, x.[f] = x) →
-    ∀ f, (counter_read x).[f] = counter_read x.
+    (∀ f, x.[f] = x) → ∀ f, (counter_read x).[f] = counter_read x.
   Proof. intros H1 f. asimpl. unfold counter_read. by rewrite ?H1. Qed.
 
   Lemma counter_read_subst (x: expr) f :
-  (counter_read x).[f] = counter_read x.[f].
+    (counter_read x).[f] = counter_read x.[f].
   Proof. unfold counter_read. by asimpl. Qed.
 
   Lemma steps_counter_read N E ρ j K x n :
     nclose N ⊆ E →
     Spec_ctx N ρ ★ x ↦ₛ (♯v n)
                ★ j ⤇ fill K (App (counter_read (Loc x)) Unit)
-      ={E}=> j ⤇ fill K (♯ n) ★ x ↦ₛ (♯v n).
+    ={E}=> j ⤇ fill K (♯ n) ★ x ↦ₛ (♯v n).
   Proof.
     intros HNE. iIntros "[#Hspec [Hx Hj]]". unfold counter_read.
-    iPvs (step_lam _ _ _ j K _ _ _ _ with "[Hj]") as "Hj"; eauto.
+    iPvs (step_lam _ _ _ j K _ Unit with "[Hj]") as "Hj"; eauto.
     asimpl.
-    iPvs (step_load _ _ _ j K _ _ _ _ with "[Hj Hx]") as "[Hj Hx]"; eauto.
-    iFrame "Hspec Hj"; trivial.
-    iPvsIntro. iFrame "Hj Hx"; trivial.
-    Unshelve. all: trivial.
+    iPvs (step_load _ _ _ j K with "[Hj Hx]") as "[Hj Hx]"; eauto.
+    { by iFrame "Hspec Hj". }
+    iPvsIntro. by iFrame "Hj Hx".
   Qed.
 
   Opaque counter_read.
-
-  Definition CG_counter_body (x l : expr) : expr :=
-    Pair (CG_locked_increment x l) (counter_read x).
 
   Lemma CG_counter_body_type x l Γ :
     typed Γ x (Tref TNat) →
     typed Γ l LockType →
     typed Γ (CG_counter_body x l)
-          (TProd (TArrow TUnit TUnit) (TArrow TUnit TNat)).
+            (TProd (TArrow TUnit TUnit) (TArrow TUnit TNat)).
   Proof.
     intros H1 H2; repeat econstructor;
       eauto using CG_locked_increment_type, counter_read_type.
   Qed.
 
   Lemma CG_counter_body_closed (x l : expr) :
-    (∀ f, x.[f] = x) →
-    (∀ f, l.[f] = l) →
+    (∀ f, x.[f] = x) → (∀ f, l.[f] = l) →
     ∀ f, (CG_counter_body x l).[f] = CG_counter_body x l.
   Proof.
     intros H1 H2 f. asimpl.
     rewrite CG_locked_increment_closed; trivial. by rewrite counter_read_closed.
   Qed.
-
-  Definition CG_counter : expr :=
-    App (Lam (App (Lam (CG_counter_body (Var 1) (Var 3)))
-                  (Alloc (♯ 0)))) newlock.
 
   Lemma CG_counter_type Γ :
     typed Γ CG_counter (TProd (TArrow TUnit TUnit) (TArrow TUnit TNat)).
@@ -199,17 +208,6 @@ Section CG_Counter.
   Qed.
 
   (* Fine-grained increment *)
-  Definition FG_increment (x : expr) : expr :=
-    Lam (App (Lam
-                (* try increment *)
-                (If (CAS x.[ren (+4)] (Var 1) (BinOp Add (♯ 1) (Var 1)))
-                    Unit (* increment succeeds we return unit *)
-                    (App (Var 2) (Var 3)) (* increment fails, we try again *)
-                )
-             )
-             (Load x.[ren (+2)]) (* read the counter *)
-        ).
-
   Lemma FG_increment_type x Γ :
     typed Γ x (Tref TNat) →
     typed Γ (FG_increment x) (TArrow TUnit TUnit).
@@ -228,13 +226,10 @@ Section CG_Counter.
     (∀ f, x.[f] = x) → ∀ f, (FG_increment x).[f] = FG_increment x.
   Proof. intros H f. asimpl. unfold FG_increment. rewrite ?H; trivial. Qed.
 
-  Definition FG_counter_body (x : expr) : expr :=
-    Pair (FG_increment x) (counter_read x).
-
   Lemma FG_counter_body_type x Γ :
     typed Γ x (Tref TNat) →
     typed Γ (FG_counter_body x)
-          (TProd (TArrow TUnit TUnit) (TArrow TUnit TNat)).
+            (TProd (TArrow TUnit TUnit) (TArrow TUnit TNat)).
   Proof.
     intros H1; econstructor.
     - apply FG_increment_type; trivial.
@@ -249,9 +244,6 @@ Section CG_Counter.
     rewrite ?H1. by rewrite counter_read_closed.
   Qed.
 
-  Definition FG_counter : expr :=
-    App (Lam (FG_counter_body (Var 1))) (Alloc (♯ 0)).
-
   Lemma FG_counter_type Γ :
     typed Γ FG_counter (TProd (TArrow TUnit TUnit) (TArrow TUnit TNat)).
   Proof.
@@ -259,8 +251,7 @@ Section CG_Counter.
     constructor. apply FG_counter_body_type; by constructor.
   Qed.
 
-  Lemma FG_counter_closed f :
-    FG_counter.[f] = FG_counter.
+  Lemma FG_counter_closed f : FG_counter.[f] = FG_counter.
   Proof. asimpl; rewrite counter_read_subst; by asimpl. Qed.
 
   Ltac prove_disj N n n' :=
@@ -269,63 +260,56 @@ Section CG_Counter.
     assert (Hneq : n ≠ n') by omega;
     set (Hdsj := ndot_ne_disjoint N n n' Hneq); set_solver_ndisj.
 
-  Lemma FG_CG_counter_refinement N Δ
-        {HΔ : ∀ x v, PersistentP (Δ x v)}
-    :
-      (@bin_log_related _ _ _ N Δ [] FG_counter CG_counter
-                        (TProd (TArrow TUnit TUnit) (TArrow TUnit TNat)) HΔ).
+  Lemma FG_CG_counter_refinement N Δ {HΔ : ∀ x v, PersistentP (Δ x v)} :
+    (@bin_log_related _ _ _ N Δ [] FG_counter CG_counter
+                      (TProd (TArrow TUnit TUnit) (TArrow TUnit TNat)) HΔ).
   Proof.
     (* executing the preambles *)
-    intros vs Hlen. destruct vs; [|inversion Hlen].
+    intros [|v vs] Hlen; simplify_eq.
     cbn -[FG_counter CG_counter].
-    intros ρ j K. iIntros "[#Hheap [#Hspec [_ Hj]]]".
-    rewrite ?empty_env_subst.
-    unfold CG_counter, FG_counter.
+    iIntros {ρ j K} "(#Hheap & #Hspec & _ & Hj)".
+    rewrite ?empty_env_subst /CG_counter /FG_counter.
     iPvs (steps_newlock _ _ _ j (K ++ [AppRCtx (LamV _)]) _ with "[Hj]")
       as {l} "[Hj Hl]"; eauto.
-    rewrite fill_app; simpl.
-    iFrame "Hspec Hj"; trivial.
-    rewrite fill_app; simpl.
+    { rewrite fill_app /=. by iFrame. }
+    rewrite fill_app /=.
     iPvs (step_lam _ _ _ j K _ _ _ _ with "[Hj]") as "Hj"; eauto.
-    asimpl. rewrite CG_locked_increment_subst; simpl.
-    rewrite counter_read_subst; simpl.
+    asimpl. rewrite CG_locked_increment_subst /=.
+    rewrite counter_read_subst /=.
     iPvs (step_alloc _ _ _ j (K ++ [AppRCtx (LamV _)]) _ _ _ _ with "[Hj]")
       as {cnt'} "[Hj Hcnt']"; eauto.
-    rewrite fill_app; simpl.
-    iFrame "Hspec Hj"; trivial.
+    { rewrite fill_app; simpl. by iFrame. }
     rewrite fill_app; simpl.
     iPvs (step_lam _ _ _ j K _ _ _ _ with "[Hj]") as "Hj"; eauto.
-    asimpl. rewrite CG_locked_increment_subst; simpl.
-    rewrite counter_read_subst; simpl.
+    asimpl. rewrite CG_locked_increment_subst /=.
+    rewrite counter_read_subst /=.
     Unshelve.
     all: try match goal with |- to_val _ = _ => auto using to_of_val end.
     all: trivial.
     iApply (@wp_bind _ _ _ [AppRCtx (LamV _)]);
       iApply wp_wand_l; iSplitR; [iIntros {v} "Hv"; iExact "Hv"|].
-    iApply wp_alloc; trivial; iFrame "Hheap"; iNext; iIntros {cnt} "Hcnt".
-    simpl.
+    iApply wp_alloc; trivial; iFrame "Hheap"; iNext; iIntros {cnt} "Hcnt /=".
     (* establishing the invariant *)
     iAssert ((∃ n, l ↦ₛ (♭v false) ★ cnt ↦ᵢ (♯v n) ★ cnt' ↦ₛ (♯v n) )%I)
       with "[Hl Hcnt Hcnt']" as "Hinv".
-    { iExists _. iFrame "Hl Hcnt Hcnt'"; trivial. }
+    { iExists _. by iFrame. }
     iPvs (inv_alloc (N .@ 4) with "[Hinv]") as "#Hinv"; trivial.
     { iNext; iExact "Hinv". }
     (* splitting increment and read *)
     iApply wp_lam; trivial. iNext. asimpl.
-    rewrite counter_read_subst; simpl.
+    rewrite counter_read_subst /=.
     iApply wp_value; simpl.
-    { rewrite counter_read_to_val; trivial. }
-    iExists (PairV (CG_locked_incrementV _ _) (counter_readV _)).
-    simpl. rewrite CG_locked_increment_of_val counter_read_of_val.
+    { by rewrite counter_read_to_val. }
+    iExists (PairV (CG_locked_incrementV _ _) (counter_readV _)); simpl.
+    rewrite CG_locked_increment_of_val counter_read_of_val.
     iFrame "Hj".
-    iExists (_, _), (_, _). simpl; repeat iSplit; trivial.
+    iExists (_, _), (_, _); simpl; repeat iSplit; trivial.
     - (* refinement of increment *)
       iAlways. clear j K. iIntros {j K v} "[#Heq Hj]".
-      rewrite CG_locked_increment_of_val. simpl.
-      destruct v; iDestruct "Heq" as "[% %]"; simpl in *;subst.
+      rewrite CG_locked_increment_of_val /=.
+      destruct v; iDestruct "Heq" as "[% %]"; simplify_eq/=.
       iLöb as "Hlat".
-      iApply wp_lam; trivial. asimpl.
-      iNext.
+      iApply wp_lam; trivial. asimpl. iNext.
       (* fine-grained reads the counter *)
       iApply (@wp_bind _ _ _ [AppRCtx (LamV _)]);
         iApply wp_wand_l; iSplitR; [iIntros {v} "Hv"; iExact "Hv"|].
@@ -344,7 +328,7 @@ Section CG_Counter.
         iApply wp_wand_l; iSplitR; [iIntros {v} "Hv"; iExact "Hv"|].
       iInv> (N .@4) as {n'} "[Hl [Hcnt Hcnt']]".
       (* performing CAS *)
-      destruct (eq_nat_dec n n') as [|Hneq]; subst.
+      destruct (decide (n = n')) as [|Hneq]; subst.
       + (* CAS succeeds *)
         (* In this case, we perform increment in the coarse-grained one *)
         iPvs (steps_CG_locked_increment
@@ -355,7 +339,7 @@ Section CG_Counter.
         iNext; iFrame "Hcnt"; iIntros "Hcnt".
         iSplitL "Hl Hcnt Hcnt'"; [iExists _; iFrame "Hl Hcnt Hcnt'"; trivial|].
         iApply wp_if_true. iNext. iApply wp_value; trivial.
-        iExists _; iSplitL; [|iSplit]; trivial. simpl; trivial.
+        iExists UnitV; iFrame; auto.
       + (* CAS fails *)
         (* In this case, we perform a recursive call *)
         iApply (wp_cas_fail _ _ _ _ (♯v n')); simpl; trivial;
@@ -367,21 +351,20 @@ Section CG_Counter.
     - (* refinement of read *)
       iAlways. clear j K. iIntros {j K v} "[#Heq Hj]".
       rewrite ?counter_read_of_val.
-      destruct v; iDestruct "Heq" as "[% %]".
-      simpl in *; subst; simpl.
+      iDestruct "Heq" as "[% %]"; destruct v; simplify_eq/=.
       Transparent counter_read.
       unfold counter_read at 2.
       iApply wp_lam; trivial. simpl.
       iNext.
       iInv> (N .@4) as {n} "[Hl [Hcnt Hcnt']]".
-      iPvs (steps_counter_read
-              _ _ _ _ _ _ _ _ with "[Hj Hcnt']") as "[Hj Hcnt']".
+      iPvs (steps_counter_read (N .@ 3) with "[Hj Hcnt']") as "[Hj Hcnt']".
+      { prove_disj N 3 4. }
       { by iFrame "Hspec Hcnt' Hj". }
       iApply wp_load; [|iFrame "Hheap"].
       { abstract prove_disj N 2 4. }
-      iNext. iFrame "Hcnt"; iIntros "Hcnt".
+      iFrame "Hcnt"; iIntros "> Hcnt".
       iSplitL "Hl Hcnt Hcnt'"; [iExists _; iFrame "Hl Hcnt Hcnt'"; trivial|].
-      iExists (♯v _); iFrame "Hj". iExists _; by iSplit.
+      iExists (♯v _); eauto.
       Unshelve.
       all: abstract prove_disj N 3 4.
   Qed.
